more locale stuff + code exportation for a constant

Weidenbach_Book/CDCL_Two_Watched_Literals_Implementation.thy
@@ -7,7 +7,17 @@ section \<open>Implementation for 2 Watched-Literals\<close>
 theory CDCL_Two_Watched_Literals_Implementation
 imports CDCL_Two_Watched_Literals DPLL_CDCL_W_Implementation
 begin
-term foldl
+
+subsection \<open>Abstract Implementation\<close>
+
+text \<open>We define here a locale serving as proxy between the abstract transition defined using
+  multiset and a more concrete version using a representation that can be converted to lists.
+  \<close>
+
+subsubsection \<open>An Extend State\<close>
+
+text \<open>The more concrete state has some way to find candidates. This is abstracted, since it can be
+  integrated to the data-structure (see 2-watched literals) \<close>
 locale conc_state\<^sub>W_with_candidates =
   state\<^sub>W trail init_clss learned_clss backtrack_lvl conflicting cons_trail tl_trail add_init_cls
    add_learned_cls remove_cls update_backtrack_lvl update_conflicting init_state
@@ -52,14 +62,15 @@ locale conc_state\<^sub>W_with_candidates =
 
     st_of_raw :: "'conc_st \<Rightarrow> 'st" and
     cls_of_raw_cls :: "'cls \<Rightarrow> 'v clause" and
-    clss_of_raw_clss :: "'clss \<Rightarrow> 'v clauses" and
+    clss_of_raw_clss :: "'clss \<Rightarrow> 'v clause list" and
     raw_cls_union :: "'cls \<Rightarrow> 'cls \<Rightarrow> 'cls" and
     remdups_raw_cls :: "'cls \<Rightarrow> 'cls" and
-    marked_lit_of_raw :: "'conc_st \<Rightarrow> 'marked_lit \<Rightarrow> ('v, nat, 'v clause) marked_lit"
+    marked_lit_of_raw :: "'marked_lit \<Rightarrow> ('v, nat, 'v clause) marked_lit" and
+    raw_marked_lit_of_marked_lit :: "('v, nat, 'cls) marked_lit \<Rightarrow> 'marked_lit"
   assumes
     (* Mapping from 'cons_st to 'st *)
     raw_cons_trail[simp]:
-      "\<And>L S. st_of_raw (raw_cons_trail L S) = cons_trail (marked_lit_of_raw S L) (st_of_raw S)" and
+      "\<And>L S. st_of_raw (raw_cons_trail L S) = cons_trail (marked_lit_of_raw L) (st_of_raw S)" and
     raw_tl_trail[simp]:
       "\<And>S. st_of_raw (raw_tl_trail S) = tl_trail (st_of_raw S)" and
     raw_add_init_cls[simp]:
@@ -67,17 +78,13 @@ locale conc_state\<^sub>W_with_candidates =
     raw_add_learned_cls[simp]:
       "\<And>C S.
         st_of_raw (raw_add_learned_cls C S) = add_learned_cls (cls_of_raw_cls C) (st_of_raw S)" and
-    raw_remove_cls[simp]:
-      "\<And>C S. distinct_mset (clauses (st_of_raw S)) \<Longrightarrow>
-        cls_of_raw_cls C \<in># clauses (st_of_raw S) \<Longrightarrow>
-        st_of_raw (raw_remove_cls C S) = remove_cls (cls_of_raw_cls C) (st_of_raw S)" and
     raw_update_backtrack_lvl[simp]:
       "\<And>k S. st_of_raw (raw_update_backtrack_lvl k S) = update_backtrack_lvl k (st_of_raw S)" and
     raw_update_conflicting[simp]:
       "\<And>(C::'cls option) S. st_of_raw (raw_update_conflicting C S) =
          update_conflicting (map_option cls_of_raw_cls C) (st_of_raw S)" and
     raw_init_state:
-      "\<And>N. st_of_raw (raw_init_state N) = init_state (clss_of_raw_clss N)" and
+      "\<And>N. st_of_raw (raw_init_state N) = init_state (mset (clss_of_raw_clss N))" and
     cls_of_raw_cls_raw_cls_union[simp]:
       "distinct_mset (cls_of_raw_cls a) \<Longrightarrow>
         distinct_mset (cls_of_raw_cls b) \<Longrightarrow>
@@ -86,6 +93,11 @@ locale conc_state\<^sub>W_with_candidates =
       "cls_of_raw_cls (remdups_raw_cls a) = remdups_mset (cls_of_raw_cls a)" and
     conflicting_raw_conflicting:
       "conflicting (st_of_raw S) = map_option cls_of_raw_cls (raw_conflicting S)" and
+    marked_lit_of_raw[simp]:
+      "marked_lit_of_raw (raw_marked_lit_of_marked_lit (Propagated L C)) =
+        Propagated L (cls_of_raw_cls C)"
+      and
+
     get_conflict_candidates_empty:
       "\<And>S. get_conflict_candidates S = [] \<longleftrightarrow>
         (\<forall>D \<in># clauses (st_of_raw S). \<not> trail (st_of_raw S) \<Turnstile>as CNot D)" and
@@ -96,7 +108,7 @@ locale conc_state\<^sub>W_with_candidates =
       "\<And>S. \<forall>(L, C) \<in> set (get_propagate_candidates S). undefined_lit (trail (st_of_raw S)) L \<and>
         cls_of_raw_cls C \<in># clauses (st_of_raw S)
         \<and> trail (st_of_raw S) \<Turnstile>as CNot (cls_of_raw_cls C - {#L#}) \<and> L \<in># cls_of_raw_cls C" and
-    get_propagate_candidates_lit_empty:
+    get_propagate_candidates_empty:
       "\<And>S. get_propagate_candidates S = [] \<longleftrightarrow>
         \<not>(\<exists>C L. undefined_lit (trail (st_of_raw S)) L \<and> C + {#L#} \<in># clauses (st_of_raw S) \<and>
           trail (st_of_raw S) \<Turnstile>as CNot C)" and
@@ -109,6 +121,7 @@ locale conc_state\<^sub>W_with_candidates =
          \<not>(\<exists>L. undefined_lit (trail (st_of_raw S)) L \<and>
          atm_of L \<in> atms_of_msu (init_clss (st_of_raw S)))"
 
+subsubsection \<open>Lowering from Transitions to Functions\<close>
 locale
   cdcl\<^sub>W_cands =
    conc_state\<^sub>W_with_candidates trail init_clss learned_clss backtrack_lvl conflicting cons_trail
@@ -124,7 +137,7 @@ locale
 
    get_propagate_candidates get_conflict_candidates get_not_decided st_of_raw
    cls_of_raw_cls clss_of_raw_clss
-   raw_cls_union remdups_raw_cls marked_lit_of_raw
+   raw_cls_union remdups_raw_cls marked_lit_of_raw raw_marked_lit_of_marked_lit
   for
     trail :: "'st \<Rightarrow> ('v::linorder, nat, 'v::linorder clause) marked_lits" and
     init_clss :: "'st \<Rightarrow> 'v clauses" and
@@ -165,10 +178,11 @@ locale
 
     st_of_raw :: "'conc_st \<Rightarrow> 'st" and
     cls_of_raw_cls :: "'cls \<Rightarrow> 'v clause" and
-    clss_of_raw_clss :: "'clss \<Rightarrow> 'v clauses" and
+    clss_of_raw_clss :: "'clss \<Rightarrow> 'v clause list" and
     raw_cls_union :: "'cls \<Rightarrow> 'cls \<Rightarrow> 'cls" and
     remdups_raw_cls :: "'cls \<Rightarrow> 'cls" and
-    marked_lit_of_raw :: "'conc_st \<Rightarrow> 'marked_lit \<Rightarrow> ('v, nat, 'v clause) marked_lit"
+    marked_lit_of_raw :: "'marked_lit \<Rightarrow> ('v, nat, 'v clause) marked_lit" and
+    raw_marked_lit_of_marked_lit :: "('v, nat, 'cls) marked_lit \<Rightarrow> 'marked_lit"
 begin
 
 interpretation cdcl\<^sub>W_termination trail init_clss learned_clss backtrack_lvl conflicting cons_trail
@@ -221,6 +235,59 @@ next
      by (auto split: list.splits option.splits simp: conflicting_raw_conflicting)
   then show ?thesis
     using get_conflict_candidates_empty by auto
+qed
+
+definition do_propagate_step :: "'conc_st \<Rightarrow> 'conc_st option" where
+"do_propagate_step S =
+  (case raw_conflicting S of
+    Some _ \<Rightarrow> None
+  | None \<Rightarrow>
+      (case get_propagate_candidates S of
+        [] \<Rightarrow> None
+      | (L, C) # _ \<Rightarrow> Some (raw_cons_trail (raw_marked_lit_of_marked_lit (Propagated L C)) S)))"
+
+lemma do_propagate_step_Some:
+  assumes conf: "do_propagate_step S = Some T"
+  shows "propagate (st_of_raw S) (st_of_raw T)"
+proof (cases "conflicting (st_of_raw S)")
+  case Some
+  then show ?thesis
+    using conf by (auto simp: do_propagate_step_def conflicting_raw_conflicting
+      split: option.splits list.splits)
+next
+  case None
+  then obtain L C where
+    C: "(L, C) \<in> set (get_propagate_candidates S)" and
+    T: "T = raw_cons_trail (raw_marked_lit_of_marked_lit (Propagated L C)) S"
+     using conf unfolding do_propagate_step_def
+    by (auto split: list.splits simp: conflicting_raw_conflicting)
+  have
+    "cls_of_raw_cls C \<in># clauses (st_of_raw S)" and
+    undef: "undefined_lit (trail (st_of_raw S)) L"
+    "trail (st_of_raw S) \<Turnstile>as CNot (cls_of_raw_cls C - {#L#})" and
+    "L \<in># cls_of_raw_cls C"
+    using get_propagate_candidates_lit_in_cls C by auto
+  then show ?thesis
+    using propagate_rule[of "st_of_raw S" "trail (st_of_raw S)" "init_clss (st_of_raw S)"
+      "learned_clss (st_of_raw S)" "backtrack_lvl (st_of_raw S)" "cls_of_raw_cls C - {#L#}" L
+      "st_of_raw T"]
+      state_eq_ref T None
+    by (auto simp: conflicting_raw_conflicting)
+qed
+
+lemma do_propagate_step_None:
+  assumes conf: "do_propagate_step S = None"
+  shows "no_step propagate (st_of_raw S)"
+proof (cases "conflicting (st_of_raw S)")
+  case Some
+  then show ?thesis by auto
+next
+  case None
+  then have "get_propagate_candidates S = []"
+     using conf unfolding do_propagate_step_def
+     by (auto split: list.splits option.splits simp: conflicting_raw_conflicting)
+  then show ?thesis
+    unfolding get_propagate_candidates_empty by (force elim!: propagateE)
 qed
 
 end
@@ -304,6 +371,7 @@ interpretation cdcl\<^sub>W: state\<^sub>W
   "\<lambda>N. ([], sorted_list_of_multiset N, [], 0, None)"
   "\<lambda>(_, N, U, _). ([], N, U, 0, None)"
   by unfold_locales (auto simp: add.commute)
+
 fun find_conflict where
 "find_conflict M [] = None" |
 "find_conflict M (N # Ns) = (if (\<forall>c \<in> set N. -c \<in> lits_of M) then Some N else find_conflict M Ns)"
@@ -327,7 +395,6 @@ lemma find_conflict_sorted_list_of_multiset_2_None:
   by (metis find_conflict_sorted_list_of_multiset_None map_append set_append)
 
 declare cdcl\<^sub>W.state_simp[simp del] cdcl\<^sub>W.clauses_def[simp add]
-
 
 lemma mset_map_mset_removeAll_remove_mset:
   "C \<in> set N \<Longrightarrow> distinct (map mset N) \<Longrightarrow>
@@ -359,50 +426,6 @@ next
     qed
   have "C \<noteq> a \<longrightarrow> mset C \<noteq> mset a"
     by (metis C dist distinct.simps(2) image_eqI list.simps(9) set_ConsD set_map)
-  then show ?case
-    unfolding rall rmset H by simp
-qed
-
-lemma
-  "distinct (map mset N) \<Longrightarrow> mset C = mset x \<Longrightarrow> x \<in> set N \<Longrightarrow>
-    mset (map mset (removeAll C N)) = remove_mset (mset x) (mset (map mset N))"
-proof (induction N)
-  case Nil
-  then show ?case by simp
-next
-  case (Cons a N) note IH = this(1) and dist = this(2) and C = this(3) and x = this(4)
-  have dist': "distinct (map mset N)"
-    using dist by auto
-  have H: "mset (map mset (removeAll C N)) = remove_mset (mset C) (mset (map mset N))"
-    by (metis (no_types, lifting) C IH x count_mset_0 diff_zero
-      dist distinct.simps(2) list.simps(9) mset_map_mset_removeAll_remove_mset
-      removeAll_id replicate_mset_0 set_ConsD)
-  have rall: "mset (map mset (removeAll C (a # N))) =
-     (if C = a then {#} else {#mset a#}) + mset (map mset (removeAll C N))"
-     by (auto simp: ac_simps)
-  have rmset: "remove_mset (mset x) (mset (map mset (a # N))) =
-     (if mset C = mset a then {#} else {#mset a#}) + remove_mset (mset C) (mset (map mset N))"
-    proof -
-      { assume a1: "mset C \<noteq> mset a"
-        then have "remove_mset (mset C) (mset (map mset (a # N))) - {#mset a#} + {#mset a#}
-          = remove_mset (mset C) (mset (map mset (a # N))) - {#}"
-          by simp (* 3 ms *)
-        then have ?thesis
-          using a1 C by (simp_all add: Multiset.diff_right_commute add.commute)}
-      then show ?thesis
-        by (cases "mset C \<noteq> mset a") (auto simp: ac_simps C)
-    qed
-  have "C \<noteq> a \<longrightarrow> mset C \<noteq> mset a"
-    proof
-      assume "C \<noteq> a"
-      have "mset C \<in> mset ` set N"
-        using C dist x apply auto sorry
-      show "mset C \<noteq> mset a"
-        apply (cases "x = a")
-        using C dist apply auto[]
-        using distinct.simps(2) image_eqI list.simps(9) set_ConsD set_map
-         sorry
-    qed
   then show ?case
     unfolding rall rmset H by simp
 qed
@@ -466,47 +489,90 @@ interpretation cdcl\<^sub>W:  conc_state\<^sub>W_with_candidates
     (convert_tr M, mset (map mset N), mset (map mset U), k, map_option mset C)"
 
   mset
-  "\<lambda>N. mset (map mset N)"
+  "\<lambda>N. (map mset N)"
   "\<lambda>a b. remdups (a @ b)"
   remdups
-  "\<lambda>_. convert"
+  convert
+  id
   apply unfold_locales
-  apply (auto simp: map_tl add.commute distinct_mset_rempdups_union_mset cdcl\<^sub>W'.clauses_def)
+  apply (auto simp: map_tl add.commute distinct_mset_rempdups_union_mset cdcl\<^sub>W'.clauses_def)[10]
+  apply (auto split: option.splits simp: find_conflict_None cdcl\<^sub>W'.clauses_def)[]
   sorry
 
 
+definition truc :: "(nat, nat, nat literal list) marked_lit list \<times>
+   nat literal list list \<times>
+   nat literal list list \<times> nat \<times> nat literal list option
+   \<Rightarrow> ((nat, nat, nat literal list) marked_lit list \<times>
+       nat literal list list \<times>
+       nat literal list list \<times>
+       nat \<times> nat literal list option) option"
+  where "truc = cdcl\<^sub>W_cands.do_conflict_step  (\<lambda>(M, N, U, k, D). D) (\<lambda>C (M, N, U, k, _). (M, N, U, k, C))
+     (\<lambda>(M, N, U, S). case find_conflict M (N @ U) of None \<Rightarrow> [] | Some a \<Rightarrow> [a])"
 
-definition "do_conflict_step = cdcl\<^sub>W_cands.do_conflict_step"
-(* interpretation gcdcl\<^sub>W2: cdcl\<^sub>W_cands
+ interpretation gcdcl\<^sub>W2: cdcl\<^sub>W_cands
   trail
-  "\<lambda>S. clauses S"
-  "\<lambda>S. learned_clss S"
-  backtrack_lvl
-  conflicting
+  clauses
+  learned_clss
+  backtrack_lvl conflicting
   "\<lambda>L (M, S). (L # M, S)"
   "\<lambda>(M, S). (tl M, S)"
   "\<lambda>C (M, N, S). (M, {#C#} + N, S)"
   "\<lambda>C (M, N, U, S). (M, N, {#C#} + U, S)"
   "\<lambda>C (M, N, U, S). (M, remove_mset C N, remove_mset C U, S)"
-  "\<lambda>(k::nat) (M, N, U, _, D). (M, N, U, k, D)"
+  "\<lambda>k (M, N, (U::nat clauses), _, D). (M, N, U, k, D)"
   "\<lambda>D (M, N, U, k, _). (M, N, U, k, D)"
   "\<lambda>N. ([], N, {#}, 0, None)"
   "\<lambda>(_, N, U, _). ([], N, U, 0, None)"
-  "\<lambda>(M, N, U, a, b).
-    case find_first_unit_clause (map sorted_list_of_multiset (sorted_list_of_multiset N @ sorted_list_of_multiset U)) M of
-      None \<Rightarrow> []
-    | Some (L, a) \<Rightarrow> [(L, mset a)]"
-  "\<lambda>(M, N, U, a, b).
-    case find_conflict M (map sorted_list_of_multiset (sorted_list_of_multiset N @ sorted_list_of_multiset U)) of
-      None \<Rightarrow> []
-    | Some a \<Rightarrow> [mset a]"
-  "\<lambda>(M, N, U, a, b). find_first_unused_var (map sorted_list_of_multiset (sorted_list_of_multiset N @ sorted_list_of_multiset U)) (lits_of M)"
-  rewrites
-  "cdcl\<^sub>W_cands.do_conflict_step S = do_conflict_step S" *)
-(*   apply unfold_locales
-  sorry
-thm do_conflict_step_def gcdcl\<^sub>W2.do_conflict_step_def do_conflict_step_def
-lemmas [code] = do_conflict_step_def gcdcl\<^sub>W2.do_conflict_step_def *)
 
+  trail
+  clauses
+  learned_clss
+  backtrack_lvl
+  conflicting
+  "\<lambda>L (M, S). (L # M, S)"
+  "\<lambda>(M, S). (tl M, S)"
+  "\<lambda>C (M, N, S). (M, C # N, S)"
+  "\<lambda>C (M, N, U, S). (M, N, C # U, S)"
+  "\<lambda>C (M, N, U, S). (M, removeAll C N, removeAll C U, S)"
+  "\<lambda>(k::nat) (M, N, U, _, D). (M, N, U, k, D)"
+  "\<lambda>D (M, N, U, k, _). (M, N, U, k, D)"
+  "\<lambda>N. ([], N, [], 0, None)"
+  "\<lambda>(_, N, U, _). ([], N, U, 0, None)"
+
+  "\<lambda>(M, N, U, S).
+    case find_first_unit_clause (N @ U) M of
+      None \<Rightarrow> []
+    | Some (L, a) \<Rightarrow> [(L, a)]"
+  "\<lambda>(M, N, U, S).
+    case find_conflict M (N @ U) of
+      None \<Rightarrow> []
+    | Some a \<Rightarrow> [a]"
+  "\<lambda>(M, N, U, S). find_first_unused_var (N @ U) (lits_of M)"
+  "\<lambda>(M, N, U, k, C).
+    (convert_tr M, mset (map mset N), mset (map mset U), k, map_option mset C)"
+
+  mset
+  "\<lambda>N. (map mset N)"
+  "\<lambda>a b. remdups (a @ b)"
+  remdups
+  convert
+  id
+  rewrites
+  "cdcl\<^sub>W_cands.do_conflict_step (\<lambda>(M, N, U, k, D). D) (\<lambda>C (M, N, U, k, _). (M, N, U, k, C))
+     (\<lambda>(M, N, U, S). case find_conflict M (N @ U) of None \<Rightarrow> [] | Some a \<Rightarrow> [a])
+  = truc"
+   apply unfold_locales
+   using [[show_abbrevs = false]]
+   unfolding truc_def apply simp
+  done
+
+
+term cdcl\<^sub>W_cands.do_conflict_step
+thm truc_def
+declare [[show_abbrevs = false, show_types = true, show_sorts]]
+thm  gcdcl\<^sub>W2.do_conflict_step_def
+declare gcdcl\<^sub>W2.do_conflict_step_def[code]
+export_code gcdcl\<^sub>W2.do_conflict_step in SML
 
 end
